Hacl.Operations: and_bytes and setmask functions

crypto_hst/utils/Hacl.Operations.fst
@@ -8,6 +8,7 @@ open Hacl.Cast
 
 (* Define base types *)
 let u8 = FStar.UInt8.t
+let s8 = Hacl.UInt8.t
 let u32 = FStar.UInt32.t
 let s32 = Hacl.UInt32.t
 let bytes = Hacl.SBuffer.u8s
@@ -19,7 +20,7 @@ let rotate_right (a:s32) (b:u32{v b <= 32}) : Tot s32 =
 
 
 (* Define helper xor function *)
-val xor_bytes: output:bytes -> in1:bytes{disjoint in1 output} -> 
+val xor_bytes: output:bytes -> in1:bytes{disjoint in1 output} ->
   len:u32{v len <= length output /\ v len <= length in1} -> STL unit
   (requires (fun h -> live h output /\ live h in1))
   (ensures  (fun h0 _ h1 -> live h0 output /\ live h0 in1 /\ live h1 output /\ live h1 in1
@@ -36,12 +37,29 @@ let rec xor_bytes output in1 len =
       xor_bytes output in1 i
     end
 
+val and_bytes: output:bytes -> in1:bytes{disjoint in1 output} ->
+  len:u32{v len <= length output /\ v len <= length in1} -> STL unit
+  (requires (fun h -> live h output /\ live h in1))
+  (ensures  (fun h0 _ h1 -> live h0 output /\ live h0 in1 /\ live h1 output /\ live h1 in1
+    /\ modifies_1 output h0 h1 ))
+let rec and_bytes output in1 len =
+  if len =^ 0ul then ()
+  else
+    begin
+      let i    = FStar.UInt32.sub_mod len 1ul in
+      let in1i = Hacl.SBuffer.index in1 i in
+      let oi   = Hacl.SBuffer.index output i in
+      let oi   = Hacl.UInt8.logand in1i oi in
+      Hacl.SBuffer.upd output i oi;
+      and_bytes output in1 i
+    end
 
-val setall_aux: (b:bytes) -> (l:u32{length b = v l}) -> (x:u8) -> (pos:u32{v pos <= length b /\ v pos < pow2 32}) 
+
+val setall_aux: (b:bytes) -> (l:u32{length b = v l}) -> (x:u8) -> (pos:u32{v pos <= length b /\ v pos < pow2 32})
   -> STL unit
         (requires (fun h -> live h b))
-        (ensures  (fun h0 _ h1 -> live h1 b /\ modifies_1 b h0 h1)) 
-    
+        (ensures  (fun h0 _ h1 -> live h1 b /\ modifies_1 b h0 h1))
+
 let rec setall_aux b l v pos =
   if lt pos l then begin
     Hacl.SBuffer.upd b pos (uint8_to_sint8 v);
@@ -54,3 +72,53 @@ val setall: (b:bytes) -> (l:u32{length b = v l}) -> (x:u8)
         (requires (fun h -> live h b))
         (ensures  (fun h0 _ h1 -> live h1 b /\ modifies_1 b h0 h1))
 let setall b l v = setall_aux b l v 0ul
+
+
+
+//
+// Naive setmask
+// * Be careful, this is not length hiding because if explicitely check
+// * the position where the byte is supposed to change
+//
+
+val setmask': mask:bytes -> masklen:u32{v masklen = Hacl.SBuffer.length mask /\ v masklen < pow2 32} -> byteval1:s8 -> byteval2:s8 -> pos:u32{v pos <= v masklen} -> i:u32{v i >= 0 /\ v i < v masklen}
+  -> STL unit
+        (requires (fun h -> live h mask))
+        (ensures  (fun h0 _ h1 -> live h1 mask /\ modifies_1 mask h0 h1))
+
+let rec setmask' mask masklen b1 b2 pos i =
+  if FStar.UInt32.eq i 0ul then ()
+  else begin
+    if FStar.UInt32.lt i pos then begin
+      Hacl.SBuffer.upd mask i b1 end
+    else begin
+      Hacl.SBuffer.upd mask i b2 end;
+    setmask' mask masklen b1 b2 pos (FStar.UInt32.sub i 1ul)
+  end
+
+val setmask: mask:bytes -> masklen:u32{v masklen = Hacl.SBuffer.length mask /\ v masklen < pow2 32 /\ v masklen >= 1} -> byteval1:s8 -> byteval2:s8 -> pos:u32{v pos <= v masklen}
+  -> STL unit
+        (requires (fun h -> live h mask))
+        (ensures  (fun h0 _ h1 -> live h1 mask /\ modifies_1 mask h0 h1))
+let setmask mask masklen b1 b2 pos = setmask' mask masklen b1 b2 pos (FStar.UInt32.sub masklen 1ul)
+
+
+(* val setmask': mask:bytes -> masklen:s32 -> byteval1:s8 -> byteval2:s8 -> pos:s32 -> i:s32  *)
+(*   -> STL unit *)
+(*         (requires (fun h -> live h mask)) *)
+(*         (ensures  (fun h0 _ h1 -> live h1 mask /\ modifies_1 mask h0 h1)) *)
+
+(* let rec setmask' mask masklen byteval1 byteval2 pos i = *)
+(*   let max = S32.add pos (uint32_to_sint32 1ul) in *)
+(*   if i = masklen then () *)
+(*   else *)
+(*     let r = S8.logor (S8.logand (S8.lt_mask i pos) byteval1) *)
+(*                      (S8.logand (S8.lognot (S32.lt_mask i max)) byteval2) in *)
+(*     Hacl.SBuffer.upd mask i r; *)
+(*     setmask' mask masklen pos (S32.add i (uint32_to_sint32 1ul)) *)
+
+(* val setmask: mask:bytes -> masklen:s32 -> byteval1:s8 -> byteval2:s8 -> pos:s32 -> i:s32  *)
+(*   -> STL unit *)
+(*         (requires (fun h -> live h mask)) *)
+(*         (ensures  (fun h0 _ h1 -> live h1 mask /\ modifies_1 mask h0 h1)) *)
+(* let setmask mask masklen pos = setmask' mask masklen pos (uint32_to_sint32 0ul) *)
